protocols/ModelCheck.v
@@ -1,0 +1,162 @@
+(* DISTRIBUTION STATEMENT A. Approved for public release. Distribution is unlimited.
+ *
+ * This material is based upon work supported by the Department of the Air Force under Air Force 
+ * Contract No. FA8702-15-D-0001. Any opinions, findings, conclusions or recommendations expressed 
+ * in this material are those of the author(s) and do not necessarily reflect the views of the 
+ * Department of the Air Force.
+ * 
+ * © 2019 Massachusetts Institute of Technology.
+ * 
+ * MIT Proprietary, Subject to FAR52.227-11 Patent Rights - Ownership by the contractor (May 2014)
+ * 
+ * The software/firmware is provided to you on an As-Is basis
+ * 
+ * Delivered to the U.S. Government with Unlimited Rights, as defined in DFARS Part 252.227-7013
+ * or 7014 (Feb 2014). Notwithstanding any copyright notice, U.S. Government rights in this work are
+ * defined by DFARS 252.227-7013 or DFARS 252.227-7014 as detailed above. Use of this work other than
+ * as specifically authorized by the U.S. Government may violate any copyrights that exist in this work. *)
+
+Require Import
+        MyPrelude
+        Sets.
+
+Set Implicit Arguments.
+
+Record trsys state := {
+  Initial : state -> Prop;
+  Step : state -> state -> Prop
+}.
+
+Definition invariantFor {state} (sys : trsys state) (invariant : state -> Prop) :=
+  forall s, sys.(Initial) s
+            -> forall s', sys.(Step)^* s s'
+                          -> invariant s'.
+
+Theorem use_invariant : forall {state} (sys : trsys state) (invariant : state -> Prop) s s',
+  invariantFor sys invariant
+  -> sys.(Step)^* s s'
+  -> sys.(Initial) s
+  -> invariant s'.
+Proof.
+  firstorder.
+Qed.
+
+Theorem invariant_weaken : forall {state} (sys : trsys state)
+  (invariant1 invariant2 : state -> Prop),
+  invariantFor sys invariant1
+  -> (forall s, invariant1 s -> invariant2 s)
+  -> invariantFor sys invariant2.
+Proof.
+  unfold invariantFor; intuition eauto.
+Qed.
+
+Theorem invariant_induction : forall {state} (sys : trsys state)
+  (invariant : state -> Prop),
+  (forall s, sys.(Initial) s -> invariant s)
+  -> (forall s, invariant s -> forall s', sys.(Step) s s' -> invariant s')
+  -> invariantFor sys invariant.
+Proof.
+  unfold invariantFor; intros.
+  assert (invariant s) by eauto.
+  clear H1.
+  induction H2; eauto.
+Qed.
+
+
+Definition oneStepClosure_current {state} (sys : trsys state)
+           (invariant1 invariant2 : state -> Prop) :=
+  forall st, invariant1 st
+             -> invariant2 st.
+
+Definition oneStepClosure_new {state} (sys : trsys state)
+           (invariant1 invariant2 : state -> Prop) :=
+  forall st st', invariant1 st
+                 -> sys.(Step) st st'
+                 -> invariant2 st'.
+
+Definition oneStepClosure {state} (sys : trsys state)
+           (invariant1 invariant2 : state -> Prop) :=
+  oneStepClosure_current sys invariant1 invariant2
+  /\ oneStepClosure_new sys invariant1 invariant2.
+
+Theorem prove_oneStepClosure : forall state (sys : trsys state) (inv1 inv2 : state -> Prop),
+  (forall st, inv1 st -> inv2 st)
+  -> (forall st st', inv1 st -> sys.(Step) st st' -> inv2 st')
+  -> oneStepClosure sys inv1 inv2.
+Proof.
+  unfold oneStepClosure; tauto.
+Qed.
+
+Theorem oneStepClosure_done : forall state (sys : trsys state) (invariant : state -> Prop),
+  (forall st, sys.(Initial) st -> invariant st)
+  -> oneStepClosure sys invariant invariant
+  -> invariantFor sys invariant.
+Proof.
+  unfold oneStepClosure, oneStepClosure_current, oneStepClosure_new.
+  intuition eauto using invariant_induction.
+Qed.
+
+Inductive multiStepClosure {state} (sys : trsys state)
+  : (state -> Prop) -> (state -> Prop) -> (state -> Prop) -> Prop :=
+| MscDone : forall inv worklist,
+    oneStepClosure sys inv inv
+    -> multiStepClosure sys inv worklist inv
+| MscStep : forall inv worklist inv' inv'',
+    oneStepClosure sys worklist inv'
+    -> multiStepClosure sys (inv \cup inv') (inv' \setminus inv) inv''
+    -> multiStepClosure sys inv worklist inv''.
+
+Lemma multiStepClosure_ok' : forall state (sys : trsys state) (inv worklist inv' : state -> Prop),
+  multiStepClosure sys inv worklist inv'
+  -> (forall st, sys.(Initial) st -> inv st)
+  -> invariantFor sys inv'.
+Proof.
+  induction 1; simpl; intuition eauto using oneStepClosure_done.
+
+  apply IHmultiStepClosure.
+  intuition.
+  apply H1 in H2.
+  sets idtac.
+Qed.
+
+Theorem multiStepClosure_ok : forall state (sys : trsys state) (inv : state -> Prop),
+  multiStepClosure sys sys.(Initial) sys.(Initial) inv
+  -> invariantFor sys inv.
+Proof.
+  eauto using multiStepClosure_ok'.
+Qed.
+
+Theorem oneStepClosure_empty : forall state (sys : trsys state),
+  oneStepClosure sys (constant nil) (constant nil).
+Proof.
+  unfold oneStepClosure, oneStepClosure_current, oneStepClosure_new; intuition.
+Qed.
+
+Theorem oneStepClosure_split : forall state (sys : trsys state) st sts (inv1 inv2 : state -> Prop),
+  (forall st', sys.(Step) st st' -> inv1 st')
+  -> oneStepClosure sys (constant sts) inv2
+  -> oneStepClosure sys (constant (st :: sts)) (constant (st :: nil) \cup inv1 \cup inv2).
+Proof.
+  unfold oneStepClosure, oneStepClosure_current, oneStepClosure_new; intuition.
+
+  inversion H0; subst.
+  unfold union; simpl; tauto.
+
+  unfold union; simpl; eauto.
+
+  unfold union in *; simpl in *.
+  intuition (subst; eauto).
+Qed.
+
+Theorem singleton_in : forall {A} (x : A) rest,
+  (constant (x :: nil) \cup rest) x.
+Proof.
+  unfold union; simpl; auto.
+Qed.
+
+Theorem singleton_in_other : forall {A} (x : A) (s1 s2 : set A),
+  s2 x
+  -> (s1 \cup s2) x.
+Proof.
+  unfold union; simpl; auto.
+Qed.
